WIP: Decision making path

Compilation.thy
@@ -21,15 +21,13 @@ datatype ('proposition, 'action) clock =
   | Running 'action
   | StartDur 'action
   | EndDur   'action
-  | ExecStartSnap 'action
-  | ExecEndSnap    'action
+  | SchedStartSnap 'action
+  | SchedEndSnap    'action
 
 datatype alpha = Unit
 
 context temp_planning_problem
 begin
-
-definition prop_numbers ("p\<^sub>_" 65) where "prop_numbers \<equiv> p"
 
 abbreviation "N \<equiv> card props"
 
@@ -44,7 +42,9 @@ fun invs::"(('proposition, 'action) clock, 'time, ('proposition, 'action, 'snap_
   "invs Main  = GE Stop 0"
 | "invs _     = EQ Stop 0"
 
-abbreviation "prop_list S \<equiv> sorted_key_list_of_set (inv p) S"
+abbreviation "prop_numbers S \<equiv> {n| n pr. n < N \<and> pr \<in> S \<and> (p n) = pr}"
+
+definition "prop_list S \<equiv> map p (sorted_list_of_set (prop_numbers S))"
 
 text \<open>The transition from the initial location \<open>l\<^sub>I\<close> to the main location \<open>l\<^sub>\<delta>\<close>\<close>
 definition init_pos::"'proposition list" where
@@ -85,19 +85,17 @@ definition exec_decoding_to_decision_making::"(alpha, ('proposition, 'action) cl
 "exec_decoding_to_decision_making \<equiv> (ExecDecoding (act M), true_const, Unit, [], Decision (at_start (act 0)))"
 
 subsubsection \<open>Decision-making\<close>
-definition AND_ALL::"(('proposition, 'action) clock, 'time) dconstraint list \<Rightarrow> (('proposition, 'action) clock, 'time) dconstraint" where
-"AND_ALL xs = fold AND xs (true_const)"
 
 text \<open>Interfering snap-actions\<close>
 
 definition interfering_at_start::"'snap_action \<Rightarrow> nat list" where
-"interfering_at_start a = sorted_list_of_set {n. mutex_snap_action a (at_start (act n))}"
+"interfering_at_start a = sorted_list_of_set {n. n < M \<and> (mutex_snap_action a (at_start (act n)) \<or> a = at_start (act n))}"
 
 definition start_constraints::"'snap_action \<Rightarrow> (('proposition, 'action) clock, 'time) dconstraint list" where
 "start_constraints a = map (\<lambda>b. GE (StartDur (act b)) \<delta>) (interfering_at_start a)"
 
 definition interfering_at_end::"'snap_action \<Rightarrow> nat list" where
-"interfering_at_end a = sorted_list_of_set {n. mutex_snap_action a (at_end (act n))}"
+"interfering_at_end a = sorted_list_of_set {n. n < M \<and> (mutex_snap_action a (at_end (act n)) \<or> a = at_end (act n))}"
 
 definition end_constraints::"'snap_action \<Rightarrow> (('proposition, 'action) clock, 'time) dconstraint list" where
 "end_constraints a = map (\<lambda>b. GE (EndDur (act b)) \<delta>) (interfering_at_end a)"
@@ -132,10 +130,10 @@ AND (AND (guard (at_end a)) (EQ (Running a) 1)) (AND l u)"
 
 definition decision_making::"(alpha, ('proposition, 'action) clock, 'time, ('proposition, 'action, 'snap_action) location) transition set" where
 "decision_making \<equiv> 
-  {(Decision (at_start (act m)), guard (at_start (act m)), Unit, [(ExecStartSnap (act m), 1)], Decision (at_end (act m))) | m. m < M}
-  \<union> {(Decision (at_start (act m)), true_const, Unit, [(ExecStartSnap (act m), 0)], Decision (at_end (act m))) | m. m < M}
-  \<union> {(Decision (at_end (act m)), guard (at_end (act m)), Unit, [(ExecEndSnap (act m), 1)], Decision (at_start (act (Suc m)))) | m. Suc m < M}
-  \<union> {(Decision (at_end (act m)), true_const, Unit, [(ExecEndSnap (act m), 0)], Decision (at_start (act (Suc m)))) | m. Suc m < M}"
+  {(Decision (at_start (act m)), guard_at_start (act m), Unit, [(SchedStartSnap (act m), 1)], Decision (at_end (act m))) | m. m < M}
+  \<union> {(Decision (at_start (act m)), true_const, Unit, [(SchedStartSnap (act m), 0)], Decision (at_end (act m))) | m. m < M}
+  \<union> {(Decision (at_end (act m)), guard_at_end (act m), Unit, [(SchedEndSnap (act m), 1)], Decision (at_start (act (Suc m)))) | m. m < M}
+  \<union> {(Decision (at_end (act m)), true_const, Unit, [(SchedEndSnap (act m), 0)], Decision (at_start (act (Suc m)))) | m. m < M}"
 
 definition dm_to_exec::"(alpha, ('proposition, 'action) clock, 'time, ('proposition, 'action, 'snap_action) location) transition" where
 "dm_to_exec \<equiv> (Decision (at_end (act M)), true_const, Unit, [], Execution (at_start (act 0)))"
@@ -159,9 +157,9 @@ definition at_end_effects::"'action \<Rightarrow> (('proposition, 'action) clock
 
 definition execution::"(alpha, ('proposition, 'action) clock, 'time, ('proposition, 'action, 'snap_action) location) transition set" where
 "execution \<equiv> 
-  {(Execution (at_start (act m)), EQ (ExecStartSnap (act m)) 1, Unit, at_start_effects (act m), Execution (at_end (act m))) | m. m < M}
+  {(Execution (at_start (act m)), EQ (SchedStartSnap (act m)) 1, Unit, at_start_effects (act m), Execution (at_end (act m))) | m. m < M}
   \<union> {(Execution (at_start (act m)), true_const, Unit, [], Execution (at_end (act m))) | m. m < M}
-  \<union> {(Execution (at_end (act m)), EQ (ExecEndSnap (act m)) 1, Unit, at_end_effects (act m), Execution (at_end (act (Suc m)))) | m. m < M}
+  \<union> {(Execution (at_end (act m)), EQ (SchedEndSnap (act m)) 1, Unit, at_end_effects (act m), Execution (at_end (act (Suc m)))) | m. m < M}
   \<union> {(Execution (at_end (act m)), true_const, Unit, [], Decision (at_start (act (Suc m)))) | m. m < M}"
 (* To do: again, a non-existent action is being accessed
 The benefit here is that there is no need to change the indexing to {0..<2M} *)
@@ -290,7 +288,7 @@ qed
 lemma last_ies_empty:
   assumes pap: "plan_actions_in_problem"
       and dnz: "durations_positive"
-      and fp:  "finite_plan"
+      and fpl:  "finite_plan"
   shows "IES (time_index (length htpl - 1)) = {}" (is "IES ?te = {}")
 proof -
   have "a \<notin> IES ?te" for a
@@ -344,7 +342,7 @@ proof -
     qed
     moreover
     
-    from d(1) set_htpl_eq_htps[OF fp] htps_def
+    from d(1) set_htpl_eq_htps[OF fpl] htps_def
     have "s + d \<in> set htpl" by blast
     ultimately
     show False using \<open>s + d > ?te\<close> by fastforce
@@ -484,7 +482,7 @@ lemma a_in_b_last_now: "a \<in> B t \<Longrightarrow> last_snap_exec' a t = t"
   by (auto intro: Greatest_equality)
 
 lemma subseq_last_snap_exec:
-  assumes fp: finite_plan
+  assumes fpl: finite_plan
       and llen: "(Suc l) < length htpl" 
 shows "last_snap_exec a (time_index (Suc l)) = last_snap_exec' a (time_index l)"
 proof -
@@ -1179,30 +1177,30 @@ proof -
   show ?thesis using steps_trans[OF W'(1) W''(1)] W'' pmW'' invW'' by blast
 qed
 
-definition exec_start_snap_corr::"(('proposition, 'action) clock, 'time) cval 
+definition start_snap_sched_corr::"(('proposition, 'action) clock, 'time) cval 
   \<Rightarrow> 'snap_action state 
   \<Rightarrow> 'action 
   \<Rightarrow> bool" where
-"exec_start_snap_corr W Q a \<equiv> (W (ExecStartSnap a) = 1 \<longleftrightarrow> (at_start a) \<in> Q) 
-  \<and> (W (ExecStartSnap a) = 0 \<longleftrightarrow> (at_start a) \<notin> Q)"
+"start_snap_sched_corr W Q a \<equiv> (W (SchedStartSnap a) = 1 \<longleftrightarrow> (at_start a) \<in> Q) 
+  \<and> (W (SchedStartSnap a) = 0 \<longleftrightarrow> (at_start a) \<notin> Q)"
 
-definition exec_end_snap_corr::"(('proposition, 'action) clock, 'time) cval 
+definition end_snap_sched_corr::"(('proposition, 'action) clock, 'time) cval 
   \<Rightarrow> 'snap_action state 
   \<Rightarrow> 'action 
   \<Rightarrow> bool" where
-"exec_end_snap_corr W Q a \<equiv> (W (ExecEndSnap a) = 1 \<longleftrightarrow> (at_start a) \<in> Q) 
-  \<and> (W (ExecEndSnap a) = 0 \<longleftrightarrow> (at_start a) \<notin> Q)"
+"end_snap_sched_corr W Q a \<equiv> (W (SchedEndSnap a) = 1 \<longleftrightarrow> (at_end a) \<in> Q) 
+  \<and> (W (SchedEndSnap a) = 0 \<longleftrightarrow> (at_end a) \<notin> Q)"
 
-definition snap_execution_state_correct::"(('proposition, 'action) clock, 'time) cval 
+definition snap_exec_sched_corr::"(('proposition, 'action) clock, 'time) cval 
   \<Rightarrow> 'snap_action state
   \<Rightarrow> bool" where
-"snap_execution_state_correct W Q \<equiv> \<forall>a \<in> actions. exec_start_snap_corr W Q a \<and> exec_end_snap_corr W Q a"
+"snap_exec_sched_corr W Q \<equiv> \<forall>a \<in> actions. start_snap_sched_corr W Q a \<and> end_snap_sched_corr W Q a"
 
 
-fun is_snap_exec_clock::"('proposition, 'action) clock \<Rightarrow> bool" where
-  "is_snap_exec_clock (ExecStartSnap _) = True"
-| "is_snap_exec_clock (ExecEndSnap _) = True"
-| "is_snap_exec_clock _ = False"
+fun is_snap_dec_clock::"('proposition, 'action) clock \<Rightarrow> bool" where
+  "is_snap_dec_clock (SchedStartSnap _) = True"
+| "is_snap_dec_clock (SchedEndSnap _) = True"
+| "is_snap_dec_clock _ = False"
 
 definition decision_making_automaton ("\<T> dm") where
 "decision_making_automaton = (decision_making \<union> {dm_to_exec}, invs)"
@@ -1212,16 +1210,316 @@ lemma decision_making:
       and MS_valid: "valid_state_sequence MS"
       and prop_clocks: "prop_model W (MS l)"
       and exec_clocks: "exec_model W (ES (time_index l))"
-      and start_durs: "\<forall>a. W (StartDur a) = exec_time (at_start a) (time_index l)"
-      and end_durs: "\<forall>a. W (EndDur a) = exec_time (at_end a) (time_index l)"
+      and start_durs: "\<forall>a \<in> actions. W (StartDur a) = exec_time (at_start a) (time_index l)"
+      and end_durs: "\<forall>a \<in> actions. W (EndDur a) = exec_time (at_end a) (time_index l)"
       and stop: "W Stop = 0"
+      and nm: "nm_happ_seq plan_happ_seq"
+      and fpl: finite_plan
+      and no_self_overlap: no_self_overlap
+      and durations_positive: durations_positive
+      and plan_actions_in_problem: plan_actions_in_problem
   shows "\<exists>W'. \<T> \<turnstile> \<langle>Decision (at_start (act 0)), W\<rangle> \<rightarrow>* \<langle>Decision (at_start (act M)), W'\<rangle> 
-    \<and> snap_execution_state_correct W (B (time_index l))
-    \<and> (\<forall>c. \<not>(is_snap_exec_clock c) \<longrightarrow> W c = W' c)"
+    \<and> snap_exec_sched_corr W (B (time_index l))
+    \<and> (\<forall>c. \<not>(is_snap_dec_clock c) \<longrightarrow> W c = W' c)"
 proof -
-  {
+  have W_sat_guard: "W \<turnstile> guard snap" 
+       if snap_in_B: "snap \<in> B (time_index l)"
+      and prop_clocks: "prop_model W (MS l)"
+      and exec_clocks: "exec_model W (ES (time_index l))" 
+      and start_durs: "\<forall>a \<in> actions. W (StartDur a) = exec_time (at_start a) (time_index l)"
+      and end_durs: "\<forall>a \<in> actions. W (EndDur a) = exec_time (at_end a) (time_index l)"
+      and stop: "W Stop = 0" for snap W
+  proof -
+    have "W \<turnstile> sep snap"
+    proof -
+      { fix b
+        assume b: "b \<in> set (interfering_at_start snap)"
+        hence b_in_act: "act b \<in> actions" unfolding interfering_at_start_def using act_img_actions by auto
+        have "b \<in> {n. n < M \<and> (mutex_snap_action snap (at_start (act n)) \<or> snap = at_start (act n))}" 
+          using b unfolding interfering_at_start_def by auto
+        hence "\<delta> \<le> exec_time (at_start (act b)) (time_index l)" using exec_time_and_epsilon[OF nm snap_in_B _ fpl] by blast
+        hence "W \<turnstile> dconstraint.GE (StartDur (act b)) \<delta>" using start_durs[THEN bspec, OF b_in_act] by auto
+      }
+      hence "list_all (clock_val W) (start_constraints snap)" 
+        unfolding start_constraints_def
+        by (subst list_all_iff) auto
+      hence "W \<turnstile> AND_ALL (start_constraints snap)" using AND_ALL_iff by blast
+      moreover
+      { fix b
+        assume b: "b \<in> set (interfering_at_end snap)"
+        hence b_in_act: "act b \<in> actions" unfolding interfering_at_end_def using act_img_actions by auto
+        have "b \<in> {n. n < M \<and> (mutex_snap_action snap (at_end (act n)) \<or> snap = at_end (act n))}" 
+          using b unfolding interfering_at_end_def by auto
+        hence "\<delta> \<le> exec_time (at_end (act b)) (time_index l)" using exec_time_and_epsilon[OF nm snap_in_B _ fpl] by blast
+        hence "W \<turnstile> dconstraint.GE (EndDur (act b)) \<delta>" using end_durs b_in_act by auto
+      }
+      hence "list_all (clock_val W) (end_constraints snap)" 
+        unfolding end_constraints_def
+        by (subst list_all_iff) auto
+      hence "W \<turnstile> AND_ALL (end_constraints snap)" using AND_ALL_iff by blast
+      ultimately
+      show ?thesis unfolding sep_def using AND_ALL_iff list_all_append by blast
+    qed
+    moreover
+    have "W \<turnstile> (pre_constraint snap)"
+    proof -
+      { fix c
+        assume "c \<in> set (pre_clocks snap)"
+        then obtain pr where
+          pr: "pr \<in> set (prop_list (pre snap))"
+          and cpr: "c = PropClock pr" using pre_clocks_def by auto
+        moreover
+        have "finite (prop_numbers (pre snap))" by simp
+        ultimately
+        have pr_in_pre: "pr \<in> pre snap" using set_sorted_list_of_set unfolding prop_list_def by auto
+        hence "pr \<in> MS l" using MS_valid[simplified valid_state_sequence_def] l_len snap_in_B by (auto simp: Let_def)
+        moreover
+        have "\<exists>a \<in> actions. snap = at_start a \<or> snap = at_end a" using snap_in_B[simplified happ_at_def]  in_happ_seqE
+          plan_actions_in_problem[simplified plan_actions_in_problem_def] by blast
+        hence "pr \<in> props" using wf_acts pr_in_pre act_img_actions by auto
+        ultimately
+        have "W c = 1" using prop_clocks cpr unfolding prop_model_def by blast
+      }
+      hence "W \<turnstile> AND_ALL (map (\<lambda>c. EQ c 1) (pre_clocks snap))" 
+        unfolding AND_ALL_iff list_all_iff by auto
+      thus ?thesis using pre_constraint_def by simp
+    qed
+    ultimately
+    show "W \<turnstile> guard snap" unfolding guard_def by blast
+  qed
 
-  }
+  have at_start_step: "\<exists>W'. \<T> dm \<turnstile> \<langle>Decision (at_start (act m)), W\<rangle> \<rightarrow> \<langle>Decision (at_end (act m)), W'\<rangle>
+        \<and> (\<forall>n < (Suc m). start_snap_sched_corr W' (B (time_index l)) (act n))
+        \<and> (\<forall>n < m. end_snap_sched_corr W' (B (time_index l)) (act n))
+        \<and> (\<forall>c. \<not>(is_snap_dec_clock c) \<longrightarrow> W c = W' c)" 
+    if prop_clocks: "prop_model W (MS l)"
+    and exec_clocks: "exec_model W (ES (time_index l))"
+    and start_durs: "\<forall>a \<in> actions. W (StartDur a) = exec_time (at_start a) (time_index l)"
+    and end_durs: "\<forall>a \<in> actions. W (EndDur a) = exec_time (at_end a) (time_index l)"
+    and stop: "W Stop = 0"
+    and m: "m < M"
+    and s_snap_corr: "\<forall>n < m. start_snap_sched_corr W (B (time_index l)) (act n)"
+    and e_snap_corr: "\<forall>n < m. end_snap_sched_corr W (B (time_index l)) (act n)"
+  for W m
+  proof (cases "at_start (act m) \<in> B (time_index l)")
+    case True
+    have trans: "(Decision (at_start (act m)), guard_at_start (act m), Unit, [(SchedStartSnap (act m), 1)], Decision (at_end (act m))) \<in> trans_of \<T> dm"
+      unfolding decision_making_automaton_def decision_making_def trans_of_def using m by auto
+    
+    have guard_sat: "W \<turnstile> guard_at_start (act m)" 
+    proof -
+      have "W \<turnstile> guard (at_start (act m))" using W_sat_guard[OF True prop_clocks exec_clocks start_durs end_durs stop] .
+      moreover 
+      have "act m \<in> actions" using act_img_actions m by blast
+      hence "W (Running (act m)) = 0" using exec_clocks[simplified exec_model_def] 
+        not_executing_when_starting[OF True _ no_self_overlap durations_positive plan_actions_in_problem]
+        by blast
+      ultimately
+      show ?thesis using guard_at_start_def by auto
+    qed
+    
+    define W' where "W' = clock_set [(SchedStartSnap (act m), 1)] W" 
+    have "\<T> dm \<turnstile> \<langle>Decision (at_start (act m)), W\<rangle> \<rightarrow> \<langle>Decision (at_end (act m)), W'\<rangle>"
+      apply (rule step_a)
+      apply (rule step_a.intros[OF trans])
+        apply (rule guard_sat)
+       apply (subst inv_of_def)
+       apply (subst decision_making_automaton_def)
+      by (auto simp: stop W'_def)
+    moreover
+    {
+      have "start_snap_sched_corr W' (B (time_index l)) (act m)" using True unfolding W'_def start_snap_sched_corr_def by simp
+      moreover
+      have "\<forall>n < m. W' (SchedStartSnap (act n)) = W (SchedStartSnap (act n))" using act_inj_on[simplified inj_on_def] m unfolding W'_def by fastforce
+      hence "(\<forall>n < m. start_snap_sched_corr W' (B (time_index l)) (act n))" using s_snap_corr unfolding start_snap_sched_corr_def by auto
+      ultimately
+      have "(\<forall>n < Suc m. start_snap_sched_corr W' (B (time_index l)) (act n))" using less_antisym by blast
+    }
+    moreover
+    { 
+      have "\<forall>n < m. W' (SchedEndSnap (act n)) = W (SchedEndSnap (act n))" using act_inj_on[simplified inj_on_def] m unfolding W'_def by fastforce
+      hence "(\<forall>n < m. end_snap_sched_corr W' (B (time_index l)) (act n))" using e_snap_corr unfolding end_snap_sched_corr_def by auto
+    }
+    moreover
+    have "(\<forall>c. \<not> is_snap_dec_clock c \<longrightarrow> W c = W' c)" unfolding W'_def by simp
+    ultimately
+    show ?thesis by meson
+  next
+    case False
+    have trans: "(Decision (at_start (act m)), true_const, Unit, [(SchedStartSnap (act m), 0)], Decision (at_end (act m))) \<in> trans_of \<T> dm"
+      unfolding decision_making_automaton_def decision_making_def trans_of_def using m by auto
+    define W' where "W' = W((SchedStartSnap (act m)) := 0)"
+    have "\<T> dm \<turnstile> \<langle>Decision (at_start (act m)), W\<rangle> \<rightarrow> \<langle>Decision (at_end (act m)), W'\<rangle>"
+      apply (rule step_a)
+      apply (rule step_a.intros[OF trans])
+      by (auto simp: true_const_def inv_of_def decision_making_automaton_def stop W'_def)
+    moreover
+    {
+      have "start_snap_sched_corr W' (B (time_index l)) (act m)" using False unfolding W'_def start_snap_sched_corr_def by simp
+      moreover
+      have "\<forall>n < m. W' (SchedStartSnap (act n)) = W (SchedStartSnap (act n))" using act_inj_on[simplified inj_on_def] m unfolding W'_def by fastforce
+      hence "(\<forall>n < m. start_snap_sched_corr W' (B (time_index l)) (act n))" using s_snap_corr unfolding start_snap_sched_corr_def by auto
+      ultimately
+      have "(\<forall>n < Suc m. start_snap_sched_corr W' (B (time_index l)) (act n))" using less_antisym by blast
+    }
+    moreover
+    { 
+      have "\<forall>n < m. W' (SchedEndSnap (act n)) = W (SchedEndSnap (act n))" using act_inj_on[simplified inj_on_def] m unfolding W'_def by fastforce
+      hence "(\<forall>n < m. end_snap_sched_corr W' (B (time_index l)) (act n))" using e_snap_corr unfolding end_snap_sched_corr_def by auto
+    }
+    moreover
+    have "(\<forall>c. \<not> is_snap_dec_clock c \<longrightarrow> W c = W' c)" unfolding W'_def by simp
+    ultimately
+    show ?thesis by meson
+  qed
+
+  have at_end_step: "\<exists>W'. \<T> dm \<turnstile> \<langle>Decision (at_end (act m)), W\<rangle> \<rightarrow> \<langle>Decision (at_start (act (Suc m))), W'\<rangle>
+        \<and> (\<forall>n < (Suc m). start_snap_sched_corr W' (B (time_index l)) (act n))
+        \<and> (\<forall>n < (Suc m). end_snap_sched_corr W' (B (time_index l)) (act n))
+        \<and> (\<forall>c. \<not>(is_snap_dec_clock c) \<longrightarrow> W c = W' c)" 
+    if prop_clocks: "prop_model W (MS l)"
+    and exec_clocks: "exec_model W (ES (time_index l))"
+    and start_durs: "\<forall>a \<in> actions. W (StartDur a) = exec_time (at_start a) (time_index l)"
+    and end_durs: "\<forall>a \<in> actions. W (EndDur a) = exec_time (at_end a) (time_index l)"
+    and stop: "W Stop = 0"
+    and m: "m < M"
+    and s_snap_corr: "\<forall>n < Suc m. start_snap_sched_corr W (B (time_index l)) (act n)"
+    and e_snap_corr: "\<forall>n < m. end_snap_sched_corr W (B (time_index l)) (act n)"
+  for W m
+  proof (cases "at_start (act m) \<in> B (time_index l)")
+    case True
+    have trans: "(Decision (at_end (act m)), guard_at_end (act m), Unit, [(SchedEndSnap (act m), 1)], Decision (at_start (act (Suc m)))) \<in> trans_of \<T> dm"
+      unfolding decision_making_automaton_def decision_making_def trans_of_def using m by auto
+    
+    have guard_sat: "W \<turnstile> guard_at_end (act m)"
+    proof -
+      have m_in_acts: "act m \<in> actions" using m act_img_actions by blast
+      have "W \<turnstile> (EQ (Running (act m)) 0)" 
+      proof -
+        have "act m \<notin> ES (time_index l)" 
+          using not_executing_when_starting[OF True _ no_self_overlap durations_positive plan_actions_in_problem] m_in_acts
+          by blast
+        hence "W (Running (act m)) = 0" using exec_clocks exec_model_def m_in_acts by force
+        thus ?thesis by blast
+      qed
+      moreover
+      have "W \<turnstile> (guard (at_start (act m)))"
+      proof -
+        have "W \<turnstile> sep (at_start (act m))"
+        proof -
+          { fix b
+            assume b: "b \<in> set (interfering_at_start (at_start (act m)))"
+            hence b_in_act: "act b \<in> actions" unfolding interfering_at_start_def using act_img_actions by auto
+            have "b \<in> {n. n < M \<and> (mutex_snap_action (at_start (act m)) (at_start (act n)) \<or> at_start (act m) = at_start (act n))}" 
+              using b unfolding interfering_at_start_def by auto
+            hence "\<delta> \<le> exec_time (at_start (act b)) (time_index l)" using exec_time_and_epsilon[OF nm True _ fpl] by blast
+            hence "W \<turnstile> dconstraint.GE (StartDur (act b)) \<delta>" using start_durs b_in_act by auto
+          }
+          hence "list_all (clock_val W) (start_constraints (at_start (act m)))" 
+            unfolding start_constraints_def
+            by (subst list_all_iff) auto
+          hence "W \<turnstile> AND_ALL (start_constraints (at_start (act m)))" using AND_ALL_iff by blast
+          moreover
+          { fix b
+            assume b: "b \<in> set (interfering_at_end (at_start (act m)))"
+            hence b_in_act: "act b \<in> actions" unfolding interfering_at_end_def using act_img_actions by auto
+            have "b \<in> {n. n < M \<and> (mutex_snap_action (at_start (act m)) (at_end (act n)) \<or> at_start (act m) = at_end (act n))}" 
+              using b unfolding interfering_at_end_def by auto
+            hence "\<delta> \<le> exec_time (at_end (act b)) (time_index l)" using exec_time_and_epsilon[OF nm True _ fpl] by blast
+            hence "W \<turnstile> dconstraint.GE (EndDur (act b)) \<delta>" using end_durs b_in_act by auto
+          }
+          hence "list_all (clock_val W) (end_constraints (at_start (act m)))" 
+            unfolding end_constraints_def
+            by (subst list_all_iff) auto
+          hence "W \<turnstile> AND_ALL (end_constraints (at_start (act m)))" using AND_ALL_iff by blast
+          ultimately
+          show ?thesis unfolding sep_def using AND_ALL_iff list_all_append by blast
+        qed
+        moreover
+        have "W \<turnstile> (pre_constraint (at_start (act m)))"
+        proof -
+          { fix c
+            assume "c \<in> set (pre_clocks (at_start (act m)))"
+            then obtain pr where
+              pr: "pr \<in> set (prop_list (pre (at_start (act m))))"
+              and cpr: "c = PropClock pr" using pre_clocks_def by auto
+            moreover
+            have "finite (prop_numbers (pre (at_start (act m))))" by simp
+            ultimately
+            have pr_in_pre: "pr \<in> pre (at_start (act m))" using set_sorted_list_of_set unfolding prop_list_def by auto
+            hence "pr \<in> MS l" using MS_valid[simplified valid_state_sequence_def] l_len True by (auto simp: Let_def)
+            moreover
+            have "pr \<in> props" using wf_acts pr_in_pre m act_img_actions by fastforce
+            ultimately
+            have "W c = 1" using prop_clocks cpr unfolding prop_model_def by blast
+          }
+          hence "W \<turnstile> AND_ALL (map (\<lambda>c. EQ c 1) (pre_clocks (at_start (act m))))" 
+            unfolding AND_ALL_iff list_all_iff by auto
+          thus ?thesis using pre_constraint_def by simp
+        qed
+        ultimately
+        show "W \<turnstile> guard (at_start (act m))" unfolding guard_def by blast
+      qed
+      ultimately
+      show "W \<turnstile> guard_at_start (act m)" using guard_at_start_def by auto
+    qed
+    
+    define W' where "W' = clock_set [(SchedStartSnap (act m), 1)] W" 
+    have "\<T> dm \<turnstile> \<langle>Decision (at_start (act m)), W\<rangle> \<rightarrow> \<langle>Decision (at_end (act m)), W'\<rangle>"
+      apply (rule step_a)
+      apply (rule step_a.intros[OF trans])
+        apply (rule guard_sat)
+       apply (subst inv_of_def)
+       apply (subst decision_making_automaton_def)
+      by (auto simp: stop W'_def)
+    moreover
+    {
+      have "start_snap_sched_corr W' (B (time_index l)) (act m)" using True unfolding W'_def start_snap_sched_corr_def by simp
+      moreover
+      have "\<forall>n < m. W' (SchedStartSnap (act n)) = W (SchedStartSnap (act n))" using act_inj_on[simplified inj_on_def] m unfolding W'_def by fastforce
+      hence "(\<forall>n < m. start_snap_sched_corr W' (B (time_index l)) (act n))" using s_snap_corr unfolding start_snap_sched_corr_def by auto
+      ultimately
+      have "(\<forall>n < Suc m. start_snap_sched_corr W' (B (time_index l)) (act n))" using less_antisym by blast
+    }
+    moreover
+    { 
+      have "\<forall>n < m. W' (SchedEndSnap (act n)) = W (SchedEndSnap (act n))" using act_inj_on[simplified inj_on_def] m unfolding W'_def by fastforce
+      hence "(\<forall>n < m. end_snap_sched_corr W' (B (time_index l)) (act n))" using e_snap_corr unfolding end_snap_sched_corr_def by auto
+    }
+    moreover
+    have "(\<forall>c. \<not> is_snap_dec_clock c \<longrightarrow> W c = W' c)" unfolding W'_def by simp
+    ultimately
+    show ?thesis by meson
+  next
+    case False
+    have trans: "(Decision (at_start (act m)), true_const, Unit, [(SchedStartSnap (act m), 0)], Decision (at_end (act m))) \<in> trans_of \<T> dm"
+      unfolding decision_making_automaton_def decision_making_def trans_of_def using m by auto
+    define W' where "W' = W((SchedStartSnap (act m)) := 0)"
+    have "\<T> dm \<turnstile> \<langle>Decision (at_start (act m)), W\<rangle> \<rightarrow> \<langle>Decision (at_end (act m)), W'\<rangle>"
+      apply (rule step_a)
+      apply (rule step_a.intros[OF trans])
+      by (auto simp: true_const_def inv_of_def decision_making_automaton_def stop W'_def)
+    moreover
+    {
+      have "start_snap_sched_corr W' (B (time_index l)) (act m)" using False unfolding W'_def start_snap_sched_corr_def by simp
+      moreover
+      have "\<forall>n < m. W' (SchedStartSnap (act n)) = W (SchedStartSnap (act n))" using act_inj_on[simplified inj_on_def] m unfolding W'_def by fastforce
+      hence "(\<forall>n < m. start_snap_sched_corr W' (B (time_index l)) (act n))" using s_snap_corr unfolding start_snap_sched_corr_def by auto
+      ultimately
+      have "(\<forall>n < Suc m. start_snap_sched_corr W' (B (time_index l)) (act n))" using less_antisym by blast
+    }
+    moreover
+    { 
+      have "\<forall>n < m. W' (SchedEndSnap (act n)) = W (SchedEndSnap (act n))" using act_inj_on[simplified inj_on_def] m unfolding W'_def by fastforce
+      hence "(\<forall>n < m. end_snap_sched_corr W' (B (time_index l)) (act n))" using e_snap_corr unfolding end_snap_sched_corr_def by auto
+    }
+    moreover
+    have "(\<forall>c. \<not> is_snap_dec_clock c \<longrightarrow> W c = W' c)" unfolding W'_def by simp
+    ultimately
+    show ?thesis by meson
+  qed
+
+
 qed
 
 definition "W\<^sub>0 \<equiv> \<lambda>c. 0"
